README.md
@@ -1,3 +1,8 @@
 # References
 ### On the Complexity of Parameterized Reachability in Reconfigurable Broadcast Networks
 https://www.irif.fr/~sangnier/publis/DSTZ-FSTTCS12-long.pdf
+
+
+### Safety Verification of Wait-Only Non-Blocking Broadcast Protocols
+https://arxiv.org/abs/2403.18591
+
